

Solving (2.5) with  $B(T, T) = 0$  gives

$$B(t, T) = \frac{1 - e^{-k(T-t)}}{k}. \quad (2.6)$$

Substituting (2.6) into (2.4) gives

$$A(T, T) - A(t, T) = \int_t^T \left[ \theta(u)B(u, T) - \frac{\sigma^2 B(u, T)^2}{2} \right] du. \quad (2.7)$$

Solving (2.7) with  $A(T, T) = 0$  leads to

$$A(t, T) = \int_t^T \left[ -\theta(u)B(u, T) + \frac{\sigma^2 B(u, T)^2}{2} \right] du. \quad (2.8)$$

Fitting the observed initial forward price  $f^*(0, T)$  results

$$f^*(0, T) = -\frac{\partial}{\partial T} \log P^*(0, T) = -A_T(0, T) + B_T(0, T)r_0, \quad (2.9)$$

where  $A_T, B_T$  denote the first derivative of  $A, B$  with respect to  $T$ .

From (2.6) and (2.8) respectively, it is easy to, differentiating with respect to  $T$ , get

$$B_T = e^{-k(T-t)},$$

and

$$\begin{aligned} A_T &= \frac{\partial}{\partial T} \left( \int_t^T \left[ -\theta(u)B(u, T) + \frac{\sigma^2 B(u, T)^2}{2} \right] du \right) \\ &= -\theta(T)B(T, T) + \frac{\sigma^2 B(T, T)^2}{2} + \int_0^T \left[ -\theta(u)B_T(u, T) + \sigma^2 B_T(u, T)B(u, T) \right] du \\ &= \int_0^T \left[ -\theta(u)B_T(u, T) + \sigma^2 B_T(u, T)B(u, T) \right] du. \end{aligned}$$

Hence (2.9) becomes

$$\begin{aligned} f^*(0, T) &= r_0 B_T(0, T) - A_T(0, T) \\ &= r_0 e^{-kT} - \frac{\sigma^2}{k} \int_0^T e^{-k(T-u)} (1 - e^{-k(T-u)}) du + \int_0^T \theta(u) e^{-k(T-u)} du \\ &= r_0 e^{-kT} - \frac{\sigma^2}{2k^2} (1 - e^{-kT})^2 + \int_0^T \theta(u) e^{-k(T-u)} du \\ &= r_0 e^{-kT} - \frac{\sigma^2}{2} B(0, T)^2 + \int_0^T \theta(u) e^{-k(T-u)} du \end{aligned}$$

Setting

$$x(T) =: r_0 e^{-kT} + \int_0^T \theta(u) e^{-k(T-u)} du,$$